src/tls/HandshakeLog.fsti
@@ -40,15 +40,8 @@ open FStar.Bytes
 
 let hash = Hashing.h //18-08-31 
 
-type msg =
-| Msg of handshake
-| Msg12 of handshake12
-| Msg13 of handshake13
+include TLS.Handshake.Send 
 
-let tag_of = function
-| Msg h -> tag_of_handshake h
-| Msg12 h -> tag_of_handshake12 h
-| Msg13 h -> tag_of_handshake13 h
 
 /// Specifies which messages indicate the end of incoming flights and
 /// triggers their handshake processing.
@@ -295,41 +288,6 @@ val send_signals: s:log -> next_keys:option (bool & bool) -> complete:bool -> ST
     hashAlg h0 s == hashAlg h1 s /\
     transcript h0 s == transcript h1 s)
 
-// FRAGMENT INTERFACE
-//
-// for outgoing messages, Handshake.Log maintains
-// - an output buffer (bytes) for handshake messages
-// - the three flags below, to be echoed and cleared once the buffer is empty
-
-type id = TLSInfo.id
-
-module Range = Range // for now
-open Range
-
-// payload of a handshake fragment, to be made opaque eventually
-type fragment (i:id) = ( rg: frange i & rbytes rg )
-//let out_msg i rg b : msg i = (|rg, b|)
-
-type next_keys_use = {
-  out_appdata  : bool; // the new key enables sending AppData fragments
-  out_ccs_first: bool; // send a CCS fragment *before* installing the new key
-  out_skip_0RTT: bool; // skip void server-to-client 0RTT epoch
-}
-
-// What the HS asks the record layer to do, in that order.
-type outgoing (i:id) (* initial index *) =
-  | Outgoing:
-      send_first: option (fragment i)  -> // HS fragment to be sent (using the current id)
-      next_keys : option next_keys_use -> // the writer index increases; details included
-      complete: bool                   -> // the handshake is complete!
-      outgoing i
-
-//17-03-26 now return an outgoing result, for uniformity
-// | OutError: error -> outgoing i       // usage? send a polite Alert in case something goes wrong when preparing messages
-
-//17-03-29  these cause a mysterious error
-//let out_next_keys (#i:id) (r:outgoing i) = Outgoing? r /\ Outgoing?.next_keys r
-//let out_complete (#i:id) (r:outgoing i)  = Outgoing? r /\ Outgoing?.complete r
 
 // provides outputs to the record layer, one fragment at a time
 // never fails, in contrast with Handshake.next_fragment
